Phi_System/Phi_Type.thy
@@ -1849,12 +1849,13 @@ declare [[
 ]]
 
 \<phi>reasoner_group variants_of_type_opr = (%cutting, [%cutting, %cutting])
-  for (\<open>Type_Variant_of_the_Same_Type_Operator F F'\<close>,
-       \<open>Type_Variant_of_the_Same_Type_Operator2 F F'\<close>,
-       \<open>Type_Variant_of_the_Same_Scalar_Mul\<^sub>0 F F'\<close>,
-       \<open>Type_Variant_of_the_Same_Scalar_Mul F F'\<close>,
-       \<open>Parameter_Variant_of_the_Same_Type F F'\<close>)
-  \<open>variants_of_type_opr\<close>
+    for (\<open>Type_Variant_of_the_Same_Type_Operator F F'\<close>,
+         \<open>Type_Variant_of_the_Same_Type_Operator2 F F'\<close>,
+         \<open>Type_Variant_of_the_Same_Scalar_Mul\<^sub>0 F F'\<close>,
+         \<open>Type_Variant_of_the_Same_Scalar_Mul F F'\<close>,
+         \<open>Parameter_Variant_of_the_Same_Type F F'\<close>)
+    \<open>variants_of_type_opr\<close>
+  and variants_of_type_opr_overrided = (%cutting+10, [%cutting+10, %cutting+10]) > variants_of_type_opr \<open>\<close>
 
 (*
 lemma Parameter_Variant_of_the_Same_Type_I [\<phi>reason 1]:
@@ -1895,39 +1896,44 @@ setup \<open>
   ]
 \<close>
 
-\<phi>reasoner_ML Parameter_Variant_of_the_Same_Type 1000 (\<open>Parameter_Variant_of_the_Same_Type _ _\<close>) = \<open>
+\<phi>reasoner_ML Parameter_Variant_of_the_Same_Type %variants_of_type_opr_overrided (\<open>Parameter_Variant_of_the_Same_Type _ ?var\<close>) = \<open>
   fn (_, (ctxt, sequent)) => Seq.make (fn () =>
-    case Thm.major_prem_of sequent
-      of _ (*Trueprop*) $ (_ (*Parameter_Variant_of_the_Same_Type*) $ LHS $ Var (v,_)) =>
-          let val thy = Proof_Context.theory_of ctxt
-              exception Not_A_Phi_Type
-              fun parse lv bvs (X $ Bound i) =
-                    if i < lv then parse lv (SOME i :: bvs) X else parse lv (NONE :: bvs) X
-                | parse lv bvs (X $ Y) = parse lv (NONE :: bvs) X
-                | parse lv bvs (Abs(_,_,X)) = parse (lv+1) (map (Option.map (fn i=>i+1)) bvs) X
-                | parse lv bvs (Const(N, _)) =
-                    let val idx = Thm.maxidx_of sequent + 1
-                        val ty = Logic.incr_tvar idx (Sign.the_const_type thy N )
-                        val args = List.take (Term.binder_types ty, length bvs)
-                        val const = Const(N, ty)
-                        val (F0,bvs) = fold_index (
-                              fn (_, (SOME b, ty)) => (fn (X,bvs) => (X $ Bound b, (b,ty)::bvs))
-                               | (i, (NONE, ty)) => (fn (X,bvs) => (X $ Var (("x",idx+i),ty), bvs))
-                            ) (bvs ~~ args) (const, [])
-                        val F = fold_index (fn (i,_) => fn X =>
-                                  case AList.lookup (op =) bvs i
-                                    of SOME ty => Abs ("_", ty, X)
-                                     | NONE => raise Not_A_Phi_Type
-                                ) bvs F0
-                             |> Thm.cterm_of ctxt
-                     in Drule.infer_instantiate ctxt [(v, F)] sequent
-                     |> (fn th => @{lemma' \<open>Parameter_Variant_of_the_Same_Type A B\<close>
-                                        by (simp add: Parameter_Variant_of_the_Same_Type_def)} RS th)
-                     |> (fn th => SOME ((ctxt,th), Seq.empty))
-                    end
-           in parse 0 [] LHS
-          end
-       | _ => NONE  
+    let val (bvtys, goal) = Phi_Help.strip_meta_hhf_bvtys (Phi_Help.leading_antecedent' sequent)
+        val _ (*Trueprop*) $ (_ (*Parameter_Variant_of_the_Same_Type*) $ LHS $ var) = goal
+        val thy = Proof_Context.theory_of ctxt
+        val (Var (v, _), bargs) = strip_comb var
+        val barg_tys = map (fn x => fastype_of1 (bvtys, x)) bargs
+        exception Not_A_Phi_Type
+        fun parse lv bvs (X $ Bound i) =
+              if i < lv then parse lv (SOME i :: bvs) X else parse lv (NONE :: bvs) X
+          | parse lv bvs (X $ Y) = parse lv (NONE :: bvs) X
+          | parse lv bvs (Abs(_,_,X)) = parse (lv+1) (map (Option.map (fn i=>i+1)) bvs) X
+          | parse lv bvs (Const(N, _)) =
+              let val idx = Thm.maxidx_of sequent + 1
+                  val ty = Logic.incr_tvar idx (Sign.the_const_type thy N )
+                  val args = List.take (Term.binder_types ty, length bvs)
+                  val a_num = length args
+                  val b_num = length barg_tys
+                  val parameterize = fold_index (fn (i,_) => fn X => X $ Bound (a_num+b_num-1-i)) barg_tys
+                  val const = Const(N, ty)
+                  val (F0,bvs) = fold_index (
+                        fn (_, (SOME b, ty)) => (fn (X,bvs) => (X $ Bound b, (b,ty)::bvs))
+                         | (i, (NONE, ty)) => (fn (X,bvs) => (X $ parameterize (Var (("x",idx+i), barg_tys ---> ty)), bvs))
+                      ) (bvs ~~ args) (const, [])
+                  val F = fold_index (fn (i,_) => fn X =>
+                            case AList.lookup (op =) bvs i
+                              of SOME ty => Abs ("_", ty, X)
+                               | NONE => raise Not_A_Phi_Type
+                          ) bvs F0
+                       |> fold_rev (fn ty => fn X => Abs ("_", ty, X)) barg_tys
+                       |> Thm.cterm_of ctxt
+               in Drule.infer_instantiate ctxt [(v, F)] sequent
+               |> (fn th => @{lemma' \<open>Parameter_Variant_of_the_Same_Type A B\<close>
+                                  by (simp add: Parameter_Variant_of_the_Same_Type_def)} RS th)
+               |> (fn th => SOME ((ctxt,th), Seq.empty))
+              end
+     in parse 0 [] LHS
+    end
 ) \<close>
 
 
@@ -3480,14 +3486,17 @@ lemma
           (inj_on f (Dom (z x)) \<longrightarrow> uz' (func_mapper' (the_inv_into (Dom (z x)) f) (\<lambda>_. True) (z' y)) = x)
 \<Longrightarrow> \<g>\<e>\<t> y \<Ztypecolon> F\<^sub>3 U \<^emph>[C\<^sub>R] F\<^sub>2 R \<f>\<r>\<o>\<m> x \<Ztypecolon> F\<^sub>1 T \<^emph>[C\<^sub>W] F\<^sub>4 W  \<close>
 
-lemma [\<phi>reason_template name F\<^sub>1.ToA_mapper[]]:
+  term Type_Variant_of_the_Same_Type_Operator
+
+lemma XXX[\<phi>reason_template name F\<^sub>1.ToA_mapper[]]:
   \<open> \<p>\<r>\<e>\<m>\<i>\<s>\<e> (\<forall>x \<in> D.
       (\<forall>a \<in> Dom (z x). f a = s (apfst g (h a))) \<longrightarrow>
       f' x = (uz' o func_mapper' s (\<lambda>_. True) o z' o apfst g' o uz o func_mapper h (\<lambda>_. True) o z) x)
 \<Longrightarrow> \<g>\<u>\<a>\<r>\<d> Functional_Transformation_Functor F\<^sub>1\<^sub>4 F\<^sub>2\<^sub>3 (T \<^emph>[C\<^sub>W] W) (U \<^emph>[C\<^sub>R] R) Dom Rng pred_mapper func_mapper
-\<Longrightarrow> \<g>\<u>\<a>\<r>\<d> Functional_Transformation_Functor F\<^sub>2\<^sub>3' F\<^sub>1\<^sub>4' (U' \<^emph>[C\<^sub>R] R) (T' \<^emph>[C\<^sub>W] W') Dom' Rng' pred_mapper' func_mapper'
+\<Longrightarrow> \<g>\<u>\<a>\<r>\<d> Parameter_Variant_of_the_Same_Type (F\<^sub>1\<^sub>4 (T \<^emph>[C\<^sub>W] W)) (F\<^sub>2\<^sub>3' (T' \<^emph>[C\<^sub>W] W'))
+\<Longrightarrow> \<g>\<u>\<a>\<r>\<d> Functional_Transformation_Functor F\<^sub>2\<^sub>3' F\<^sub>1\<^sub>4' (U' \<^emph>[C\<^sub>R] R') (T' \<^emph>[C\<^sub>W] W') Dom' Rng' pred_mapper' func_mapper'
 \<Longrightarrow> \<g>\<u>\<a>\<r>\<d> Separation_Homo\<^sub>I_Cond F\<^sub>1 F\<^sub>4 F\<^sub>1\<^sub>4 C\<^sub>W T W Dz z
-\<Longrightarrow> \<g>\<u>\<a>\<r>\<d> Separation_Homo\<^sub>I_Cond F\<^sub>3' F\<^sub>2 F\<^sub>2\<^sub>3' C\<^sub>R U' R Dz' z'
+\<Longrightarrow> \<g>\<u>\<a>\<r>\<d> Separation_Homo\<^sub>I_Cond F\<^sub>3' F\<^sub>2' F\<^sub>2\<^sub>3' C\<^sub>R U' R' Dz' z'
 \<Longrightarrow> \<g>\<u>\<a>\<r>\<d> Separation_Homo\<^sub>E_Cond F\<^sub>3 F\<^sub>2 F\<^sub>2\<^sub>3 C\<^sub>R U R Du uz
 \<Longrightarrow> \<g>\<u>\<a>\<r>\<d> Separation_Homo\<^sub>E_Cond F\<^sub>1' F\<^sub>4' F\<^sub>1\<^sub>4' C\<^sub>W T' W' Du' uz'
 \<Longrightarrow> \<p>\<r>\<e>\<m>\<i>\<s>\<e> D \<subseteq> Dz \<and> (\<forall>x \<in> D. \<forall>a \<in> Dom (z x). h a \<in> Rng (z x)) \<and>
@@ -3496,20 +3505,21 @@ lemma [\<phi>reason_template name F\<^sub>1.ToA_mapper[]]:
            (\<forall>x\<in>D. Dom' (z' (apfst g' (uz (func_mapper h (\<lambda>_. True) (z x))))) = apfst g ` h ` Dom (z x)) \<and>
            (\<forall>x \<in> apfst g' ` uz ` func_mapper h (\<lambda>_. True) ` z ` D. \<forall>a \<in> Dom' (z' x). s a \<in> Rng' (z' x)) \<and>
            (\<forall>x \<in> apfst g' ` uz ` func_mapper h (\<lambda>_. True) ` z ` D. func_mapper' s (\<lambda>_. True) (z' x) \<in> Du')
-\<Longrightarrow> \<m>\<a>\<p> g  : U \<mapsto> U' \<r>\<e>\<m>\<a>\<i>\<n>\<i>\<n>\<g>[C\<^sub>R] R \<o>\<v>\<e>\<r> f : T \<^emph>[C\<^sub>W] W \<mapsto> T' \<^emph>[C\<^sub>W] W'
+\<Longrightarrow> \<m>\<a>\<p> apfst g  : U \<^emph>[C\<^sub>R] R \<mapsto> U' \<^emph>[C\<^sub>R] R' \<o>\<v>\<e>\<r> f : T \<^emph>[C\<^sub>W] W \<mapsto> T' \<^emph>[C\<^sub>W] W'
     \<w>\<i>\<t>\<h> \<g>\<e>\<t>\<t>\<e>\<r> h \<s>\<e>\<t>\<t>\<e>\<r> s \<i>\<n> \<Union> (Dom ` z ` D)
 \<Longrightarrow> \<s>\<i>\<m>\<p>\<l>\<i>\<f>\<y> h' : uz o func_mapper h (\<lambda>_. True) o z @action \<A>_template_reason
 \<Longrightarrow> \<s>\<i>\<m>\<p>\<l>\<i>\<f>\<y> s' : uz' o func_mapper' s (\<lambda>_. True) o z' @action \<A>_template_reason
-\<Longrightarrow> \<m>\<a>\<p> g' : F\<^sub>3 U \<mapsto> F\<^sub>3' U' \<r>\<e>\<m>\<a>\<i>\<n>\<i>\<n>\<g>[C\<^sub>R] F\<^sub>2 R \<o>\<v>\<e>\<r> f' : F\<^sub>1 T \<^emph>[C\<^sub>W] F\<^sub>4 W \<mapsto> F\<^sub>1' T' \<^emph>[C\<^sub>W] F\<^sub>4' W'
+\<Longrightarrow> \<m>\<a>\<p> apfst g' : F\<^sub>3 U \<^emph>[C\<^sub>R] F\<^sub>2 R \<mapsto> F\<^sub>3' U' \<^emph>[C\<^sub>R] F\<^sub>2' R' \<o>\<v>\<e>\<r> f' : F\<^sub>1 T \<^emph>[C\<^sub>W] F\<^sub>4 W \<mapsto> F\<^sub>1' T' \<^emph>[C\<^sub>W] F\<^sub>4' W'
     \<w>\<i>\<t>\<h> \<g>\<e>\<t>\<t>\<e>\<r> h' \<s>\<e>\<t>\<t>\<e>\<r> s' \<i>\<n> D\<close>
+
   unfolding \<r>Guard_def Action_Tag_def
-  \<medium_left_bracket> premises [] and FTF[] and FTF'[] and SH\<^sub>I[] and SH\<^sub>I'[] and SH\<^sub>E[] and SH\<^sub>E'[] and _ and Tr and [simp] and [simp]
+  \<medium_left_bracket> premises [] and FTF[] and [] and FTF'[] and SH\<^sub>I[] and SH\<^sub>I'[] and SH\<^sub>E[] and SH\<^sub>E'[] and _ and Tr and [simp] and [simp]
     apply_rule apply_Separation_Homo\<^sub>I_Cond[where Fu=F\<^sub>4 and Ft=F\<^sub>1, OF SH\<^sub>I]
     apply_rule apply_Functional_Transformation_Functor[where U=\<open>U \<^emph>[C\<^sub>R] R\<close> and f=\<open>h\<close> and P=\<open>\<lambda>_. True\<close>, OF FTF]
     \<medium_left_bracket> apply_rule apply_ToA_Mapper_onward[OF Tr] \<medium_right_bracket>
         apply_rule apply_Separation_Homo\<^sub>E_Cond[OF SH\<^sub>E]
   \<medium_right_bracket> apply (rule conjunctionI, simp)
-  \<medium_left_bracket> premises [] and FTF[] and FTF'[] and SH\<^sub>I[] and SH\<^sub>I'[] and SH\<^sub>E[] and SH\<^sub>E'[] and _ and Tr and [simp] and [simp]
+  \<medium_left_bracket> premises [] and FTF[] and [] and FTF'[] and SH\<^sub>I[] and SH\<^sub>I'[] and SH\<^sub>E[] and SH\<^sub>E'[] and _ and Tr and [simp] and [simp]
     apply_rule apply_Separation_Homo\<^sub>I_Cond[OF SH\<^sub>I']
     apply_rule apply_Functional_Transformation_Functor[where f=s and P=\<open>\<lambda>_. True\<close>, OF FTF']
     \<medium_left_bracket> for a
